isabelle-thys/CQ_Operators.thy
@@ -2,17 +2,16 @@ theory CQ_Operators
   imports Kraus_Maps
 begin
 
-definition \<open>program_semantics_rel \<EE> \<FF> \<longleftrightarrow> (\<forall>x. kraus_family_norm (\<EE> x) \<le> 1 \<and> kraus_equivalent' (\<EE> x) (\<FF> x))\<close>
+definition \<open>cq_map_rel \<EE> \<FF> \<longleftrightarrow> (\<forall>x. kraus_family_norm (\<EE> x) \<le> 1 \<and> kraus_equivalent' (\<EE> x) (\<FF> x))\<close>
   for \<EE> \<FF> :: \<open>'cl \<Rightarrow> ('qu ell2, 'qu ell2, 'cl) kraus_family\<close>
 
-(* TODO rename \<rightarrow> cq_operator *)
-typedef ('cl,'qu) program_state = \<open>{\<rho> :: 'cl \<Rightarrow> ('qu ell2, 'qu ell2) trace_class. (\<forall>c. \<rho> c \<ge> 0) \<and> 
+typedef ('cl,'qu) cq_operator = \<open>{\<rho> :: 'cl \<Rightarrow> ('qu ell2, 'qu ell2) trace_class. (\<forall>c. \<rho> c \<ge> 0) \<and> 
                           (\<lambda>c. trace_tc (\<rho> c)) summable_on UNIV \<and> (\<Sum>\<^sub>\<infinity>c. trace_tc (\<rho> c)) \<le> 1}\<close>
   apply (rule exI[of _ \<open>\<lambda>_. 0\<close>])
   by auto
-setup_lifting type_definition_program_state
+setup_lifting type_definition_cq_operator
 
-lift_definition fixed_cl_program_state :: \<open>'cl \<Rightarrow> ('qu ell2, 'qu ell2) trace_class \<Rightarrow> ('cl,'qu) program_state\<close> is
+lift_definition fixed_cl_cq_operator :: \<open>'cl \<Rightarrow> ('qu ell2, 'qu ell2) trace_class \<Rightarrow> ('cl,'qu) cq_operator\<close> is
   \<open>\<lambda>c (\<rho>::('qu ell2, 'qu ell2) trace_class) d. if \<rho> \<ge> 0 \<and> trace_tc \<rho> \<le> 1 then of_bool (c=d) *\<^sub>R \<rho> else 0\<close>
 proof (rename_tac c \<rho>, intro conjI allI)
   fix c d :: 'cl and \<rho> :: \<open>('qu ell2, 'qu ell2) trace_class\<close>
@@ -49,47 +48,46 @@ proof (rename_tac c \<rho>, intro conjI allI)
 qed
 
 
-(* TODO rename \<rightarrow> cq_map *)
-quotient_type ('cl,'qu) program_semantics = \<open>'cl \<Rightarrow> ('qu ell2, 'qu ell2, 'cl) kraus_family\<close> /
-  partial: program_semantics_rel
+quotient_type ('cl,'qu) cq_map = \<open>'cl \<Rightarrow> ('qu ell2, 'qu ell2, 'cl) kraus_family\<close> /
+  partial: cq_map_rel
 proof (rule part_equivpI)
-  show \<open>\<exists>x. program_semantics_rel x x\<close>
+  show \<open>\<exists>x. cq_map_rel x x\<close>
     apply (rule exI[of _ \<open>\<lambda>_. 0\<close>])
-    by (simp add: program_semantics_rel_def)
-  show \<open>symp program_semantics_rel\<close>
+    by (simp add: cq_map_rel_def)
+  show \<open>symp cq_map_rel\<close>
   proof (rule sympI)
-    fix \<EE> \<FF> assume asm: \<open>program_semantics_rel \<EE> \<FF>\<close>
+    fix \<EE> \<FF> assume asm: \<open>cq_map_rel \<EE> \<FF>\<close>
     then have eq1: \<open>kraus_equivalent' (\<EE> x) (\<FF> x)\<close> for x
-      unfolding program_semantics_rel_def by blast
+      unfolding cq_map_rel_def by blast
     then have eq2: \<open>kraus_equivalent' (\<FF> x) (\<EE> x)\<close> for x
       using kraus_equivalent'_sym by blast
     from eq1 have eq3: \<open>kraus_equivalent (\<EE> x) (\<FF> x)\<close> for x
       by (rule kraus_equivalent'_imp_equivalent)
     have \<open>kraus_family_norm (\<EE> x) \<le> 1\<close> for x
-      using asm unfolding program_semantics_rel_def by blast
+      using asm unfolding cq_map_rel_def by blast
     with eq3
     have norm: \<open>kraus_family_norm (\<FF> x) \<le> 1\<close> for x
       by (metis kraus_family_norm_welldefined)
-    with eq2 show \<open>program_semantics_rel \<FF> \<EE>\<close>
-      by (simp add: program_semantics_rel_def)
+    with eq2 show \<open>cq_map_rel \<FF> \<EE>\<close>
+      by (simp add: cq_map_rel_def)
   qed
-  show \<open>transp program_semantics_rel\<close>
-    apply (auto intro!: transpI simp: program_semantics_rel_def)
+  show \<open>transp cq_map_rel\<close>
+    apply (auto intro!: transpI simp: cq_map_rel_def)
     using kraus_equivalent'_trans by blast
 qed
-(* setup_lifting type_definition_program_semantics *)
+(* setup_lifting type_definition_cq_map *)
 
-lift_definition program_semantics_id :: \<open>('cl,'qu) program_semantics\<close> is 
+lift_definition cq_map_id :: \<open>('cl,'qu) cq_map\<close> is 
   \<open>\<lambda>c. kraus_family_map_outcome (\<lambda>(). c) kraus_family_id\<close>
-  by (simp add: program_semantics_rel_def)
+  by (simp add: cq_map_rel_def)
 
-lift_definition program_semantics_apply :: \<open>('cl,'qu) program_semantics \<Rightarrow> ('cl,'qu) program_state \<Rightarrow> ('cl,'qu) program_state\<close> is
+lift_definition cq_map_apply :: \<open>('cl,'qu) cq_map \<Rightarrow> ('cl,'qu) cq_operator \<Rightarrow> ('cl,'qu) cq_operator\<close> is
   \<open>\<lambda>\<EE> \<rho> c. (\<Sum>\<^sub>\<infinity>d. kraus_family_map' {c} (\<EE> d) (\<rho> d))\<close>
 proof (rename_tac \<EE> \<EE>' \<rho>, intro conjI allI ext)
   fix \<EE> \<EE>' :: \<open>'cl \<Rightarrow> ('qu ell2, 'qu ell2, 'cl) kraus_family\<close>
-  assume rel: \<open>program_semantics_rel \<EE> \<EE>'\<close>
+  assume rel: \<open>cq_map_rel \<EE> \<EE>'\<close>
   then have norm_\<EE>: \<open>kraus_family_norm (\<EE> x) \<le> 1\<close> for x
-    unfolding program_semantics_rel_def by blast
+    unfolding cq_map_rel_def by blast
   fix \<rho> :: \<open>'cl \<Rightarrow> ('qu ell2, 'qu ell2) trace_class\<close> and c
   assume \<open>(\<forall>c. 0 \<le> \<rho> c) \<and> (\<lambda>c. trace_tc (\<rho> c)) summable_on UNIV \<and> (\<Sum>\<^sub>\<infinity>c. trace_tc (\<rho> c)) \<le> 1\<close>
   then have \<rho>_pos: \<open>0 \<le> \<rho> c\<close> and \<rho>_sum: \<open>(\<lambda>c. trace_tc (\<rho> c)) summable_on UNIV\<close> and \<rho>_leq1: \<open>(\<Sum>\<^sub>\<infinity>c. trace_tc (\<rho> c)) \<le> 1\<close> for c
@@ -102,10 +100,10 @@ proof (rename_tac \<EE> \<EE>' \<rho>, intro conjI allI ext)
   from \<rho>_pos
   have 9: \<open>trace_tc (kraus_family_map (\<EE> d) (\<rho> d)) \<le> kraus_family_norm (\<EE> d) * trace_tc (\<rho> d)\<close> for d
     by (smt (verit) Extra_Ordered_Fields.complex_of_real_cmod cmod_mono complex_of_real_nn_iff 
-        kraus_family_map_bounded_pos kraus_family_map_pos nn_comparable norm_tc_pos of_real_hom.hom_mult 
+        kraus_family_map_bounded_pos abs_pos kraus_family_map_pos nn_comparable norm_tc_pos of_real_hom.hom_mult 
         of_real_hom.injectivity trace_tc_0 trace_tc_mono) 
   from \<rho>_pos have 10: \<open>\<dots>d \<le> trace_tc (\<rho> d)\<close> for d
-    by (smt (verit) Extra_Ordered_Fields.complex_of_real_cmod Extra_Ordered_Fields.mult_sign_intros(1) cmod_mono complex_of_real_leq_1_iff complex_of_real_nn_iff kraus_family_norm_geq0 mult_left_le_one_le nn_comparable norm_\<EE> norm_mult trace_tc_0 trace_tc_mono) 
+    by (smt (verit, del_insts) Rings.mult_sign_intros(1) cmod_Re complex_of_real_leq_1_iff complex_of_real_nn_iff kraus_family_norm_geq0 less_eq_complex_def mult_left_le_one_le norm_\<EE> norm_ge_zero norm_mult norm_one trace_tc_pos)
   have 0: \<open>0 \<le> Re (trace_tc (kraus_family_map' {c} (\<EE> d) (\<rho> d)))\<close> for c d
     by (metis Re_complex_of_real \<rho>_pos kraus_family_map'_pos norm_cblinfun_mono_trace_class norm_tc_pos norm_zero order_eq_refl)
   have 3: \<open>(\<Sum>\<^sub>\<infinity>c. kraus_family_map' {c} (\<EE> d) (\<rho> d)) = kraus_family_map (\<EE> d) (\<rho> d)\<close> for d
@@ -132,7 +130,7 @@ proof (rename_tac \<EE> \<EE>' \<rho>, intro conjI allI ext)
   have 16: \<open>bounded_linear (\<lambda>x. Re (trace_tc x))\<close> for x :: \<open>('qu ell2,'qu ell2) trace_class\<close>
     by (intro bounded_linear_compose[OF bounded_linear_Re] bounded_linear_intros)
   from 3 4 have 5: \<open>(\<Sum>\<^sub>\<infinity>c. Re (trace_tc (kraus_family_map' {c} (\<EE> d) (\<rho> d)))) = Re (trace_tc (kraus_family_map (\<EE> d) (\<rho> d)))\<close> for d
-    apply (subst infsum_bounded_linear[where f=\<open>Re o trace_tc\<close>, unfolded o_def])
+    apply (subst infsum_bounded_linear[where h=\<open>Re o trace_tc\<close>, unfolded o_def])
     using 16 by auto
   have 13: \<open>0 \<le> Re (trace_tc (kraus_family_map (\<EE> d) (\<rho> d)))\<close> for d
     by (metis Re_complex_of_real \<rho>_pos kraus_family_map_pos norm_cblinfun_mono_trace_class norm_tc_pos norm_zero order_eq_refl)
@@ -153,7 +151,7 @@ proof (rename_tac \<EE> \<EE>' \<rho>, intro conjI allI ext)
     apply (rule abs_summable_summable)
     using 12 28 by auto
   have 15: \<open>(\<Sum>\<^sub>\<infinity>d. Re (trace_tc (\<rho> d))) \<le> 1\<close>
-    apply (subst infsum_bounded_linear[where f=\<open>Re o trace_tc\<close>, unfolded o_def])
+    apply (subst infsum_bounded_linear[where h=\<open>Re o trace_tc\<close>, unfolded o_def])
     using 16 27 28 \<rho>_sum \<rho>_leq1 \<rho>_pos
       apply auto
     by (smt (verit) Infinite_Sum.infsum_nonneg_complex abs_summable_on_comparison_test cmod_mono complex_Re_le_cmod infsum_Re infsum_cong norm_infsum_bound norm_one summable_on_iff_abs_summable_on_complex trace_tc_norm trace_tc_pos)
@@ -208,65 +206,65 @@ proof (rename_tac \<EE> \<EE>' \<rho>, intro conjI allI ext)
         simp: infsum_of_real )
   from rel
   show \<open>(\<Sum>\<^sub>\<infinity>d. kraus_family_map' {c} (\<EE> d) (\<rho> d)) = (\<Sum>\<^sub>\<infinity>d. kraus_family_map' {c} (\<EE>' d) (\<rho> d))\<close>
-    by (auto intro!: kraus_family_map'_eqI infsum_cong simp: program_semantics_rel_def)
+    by (auto intro!: kraus_family_map'_eqI infsum_cong simp: cq_map_rel_def)
 qed
 
-lift_definition program_semantics_seq :: \<open>('cl,'qu) program_semantics \<Rightarrow> ('cl,'qu) program_semantics \<Rightarrow> ('cl,'qu) program_semantics\<close>
+lift_definition cq_map_seq :: \<open>('cl,'qu) cq_map \<Rightarrow> ('cl,'qu) cq_map \<Rightarrow> ('cl,'qu) cq_map\<close>
   is \<open>\<lambda>\<EE> \<FF> c. kraus_family_map_outcome snd (kraus_family_comp_dependent \<FF> (\<EE> c))\<close>
 proof -
   fix \<EE> \<FF> \<EE>' \<FF>' :: \<open>'cl \<Rightarrow> ('qu ell2, 'qu ell2, 'cl) kraus_family\<close>
-  assume asms: \<open>program_semantics_rel \<EE> \<EE>'\<close>  \<open>program_semantics_rel \<FF> \<FF>'\<close>
+  assume asms: \<open>cq_map_rel \<EE> \<EE>'\<close>  \<open>cq_map_rel \<FF> \<FF>'\<close>
   have F1: \<open>kraus_family_norm (\<FF>' x) \<le> 1\<close> for x
-    by (metis asms(2) kraus_equivalent'_imp_equivalent kraus_family_norm_welldefined program_semantics_rel_def)
+    by (metis asms(2) kraus_equivalent'_imp_equivalent kraus_family_norm_welldefined cq_map_rel_def)
   have \<open>kraus_family_norm (kraus_family_comp_dependent \<FF> (\<EE> x)) \<le> 1 * kraus_family_norm (\<EE> x)\<close> for x
     apply (rule kraus_family_comp_dependent_norm)
-    using asms(2) unfolding program_semantics_rel_def by blast
+    using asms(2) unfolding cq_map_rel_def by blast
   also have \<open>\<dots>x \<le> 1 * 1\<close> for x
-    using asms(1) program_semantics_rel_def by force
+    using asms(1) cq_map_rel_def by force
   finally have 1: \<open>kraus_family_norm (kraus_family_comp_dependent \<FF> (\<EE> x)) \<le> 1\<close> for x
     by simp
   have 2: \<open>kraus_equivalent' (kraus_family_map_outcome snd (kraus_family_comp_dependent \<FF> (\<EE> x)))
                  (kraus_family_map_outcome snd (kraus_family_comp_dependent \<FF>' (\<EE>' x)))\<close> for x
     using asms
     by (auto intro!: F1 bdd_aboveI kraus_equivalent'_map_cong kraus_family_comp_dependent_cong'
-        simp: program_semantics_rel_def)
+        simp: cq_map_rel_def)
   from 1 2
-  show \<open>program_semantics_rel (\<lambda>c. kraus_family_map_outcome snd (kraus_family_comp_dependent \<FF> (\<EE> c)))
+  show \<open>cq_map_rel (\<lambda>c. kraus_family_map_outcome snd (kraus_family_comp_dependent \<FF> (\<EE> c)))
         (\<lambda>c. kraus_family_map_outcome snd (kraus_family_comp_dependent \<FF>' (\<EE>' c)))\<close>
-    by (simp add: program_semantics_rel_def)
+    by (simp add: cq_map_rel_def)
 qed
 
-lemma program_semantics_eqI:
-  assumes \<open>\<And>\<rho>. program_semantics_apply s \<rho> = program_semantics_apply t \<rho>\<close>
+lemma cq_map_eqI:
+  assumes \<open>\<And>\<rho>. cq_map_apply s \<rho> = cq_map_apply t \<rho>\<close>
   shows \<open>s = t\<close>
 proof -
-  from assms[THEN Rep_program_state_inject[THEN iffD2]]
-  have *: \<open>(\<Sum>\<^sub>\<infinity>d. kraus_family_map' {c} (rep_program_semantics s d) (Rep_program_state \<rho> d))
-      = (\<Sum>\<^sub>\<infinity>d. kraus_family_map' {c} (rep_program_semantics t d) (Rep_program_state \<rho> d))\<close> for c \<rho>
-    apply (simp add: program_semantics_apply.rep_eq)
+  from assms[THEN Rep_cq_operator_inject[THEN iffD2]]
+  have *: \<open>(\<Sum>\<^sub>\<infinity>d. kraus_family_map' {c} (rep_cq_map s d) (Rep_cq_operator \<rho> d))
+      = (\<Sum>\<^sub>\<infinity>d. kraus_family_map' {c} (rep_cq_map t d) (Rep_cq_operator \<rho> d))\<close> for c \<rho>
+    apply (simp add: cq_map_apply.rep_eq)
     by meson
-  have \<open>kraus_family_map' {c} (rep_program_semantics s d) \<rho> = kraus_family_map' {c} (rep_program_semantics t d) \<rho>\<close>
+  have \<open>kraus_family_map' {c} (rep_cq_map s d) \<rho> = kraus_family_map' {c} (rep_cq_map t d) \<rho>\<close>
     if \<open>\<rho> \<ge> 0\<close> and \<open>trace_tc \<rho> \<le> 1\<close> for c d \<rho>
-    using *[of c \<open>fixed_cl_program_state d \<rho>\<close>]
-    unfolding fixed_cl_program_state.rep_eq
+    using *[of c \<open>fixed_cl_cq_operator d \<rho>\<close>]
+    unfolding fixed_cl_cq_operator.rep_eq
     apply (subst (asm) infsum_single[where i=d])
      apply auto[1]
     apply (subst (asm) infsum_single[where i=d])
     using that by auto
-  then have \<open>kraus_family_map' {c} (rep_program_semantics s d) = kraus_family_map' {c} (rep_program_semantics t d)\<close> for c d
+  then have \<open>kraus_family_map' {c} (rep_cq_map s d) = kraus_family_map' {c} (rep_cq_map t d)\<close> for c d
     apply (rule eq_from_separatingI[OF separating_density_ops[where B=1], rotated -1])
         apply (auto intro!: kraus_family_map'_bounded_clinear bounded_clinear.clinear)
     using complex_of_real_mono norm_tc_pos by fastforce
-  from fun_cong[OF this] have \<open>kraus_equivalent' (rep_program_semantics s c) (rep_program_semantics t c)\<close> for c
+  from fun_cong[OF this] have \<open>kraus_equivalent' (rep_cq_map s c) (rep_cq_map t c)\<close> for c
     by (rule kraus_equivalent'I)
   then show ?thesis
-    apply (rule_tac Quotient3_rel_rep[OF Quotient3_program_semantics, THEN iffD1])
-    using Quotient3_rep_reflp[OF Quotient3_program_semantics, of s]
-    using Quotient3_rep_reflp[OF Quotient3_program_semantics, of t]
-    by (simp add: program_semantics_rel_def)
+    apply (rule_tac Quotient3_rel_rep[OF Quotient3_cq_map, THEN iffD1])
+    using Quotient3_rep_reflp[OF Quotient3_cq_map, of s]
+    using Quotient3_rep_reflp[OF Quotient3_cq_map, of t]
+    by (simp add: cq_map_rel_def)
 qed
 
-lemma program_semantics_apply_id[simp]: \<open>program_semantics_apply program_semantics_id \<rho> = \<rho>\<close>
+lemma cq_map_apply_id[simp]: \<open>cq_map_apply cq_map_id \<rho> = \<rho>\<close>
 proof transfer'
   fix \<rho> :: \<open>'cl \<Rightarrow> ('qu ell2, 'qu ell2) trace_class\<close>
   have inj: \<open>inj_on (\<lambda>(). x) X\<close> for x :: 'cl and X
@@ -295,14 +293,14 @@ proof transfer'
   qed
 qed
 
-lemma program_semantics_apply_seq: \<open>program_semantics_apply (program_semantics_seq s t) \<rho> = program_semantics_apply t (program_semantics_apply s \<rho>)\<close>
+lemma cq_map_apply_seq: \<open>cq_map_apply (cq_map_seq s t) \<rho> = cq_map_apply t (cq_map_apply s \<rho>)\<close>
 proof (transfer, intro ext)
   fix s t :: \<open>'cl \<Rightarrow> ('qu ell2, 'qu ell2, 'cl) kraus_family\<close> and \<rho> :: \<open>'cl \<Rightarrow> ('qu ell2, 'qu ell2) trace_class\<close> and c :: 'cl
   assume assms: \<open>(\<forall>c. 0 \<le> \<rho> c) \<and> (\<lambda>c. trace_tc (\<rho> c)) summable_on UNIV \<and> (\<Sum>\<^sub>\<infinity>c. trace_tc (\<rho> c)) \<le> 1\<close>
-  assume \<open>program_semantics_rel s s\<close>
-  assume \<open>program_semantics_rel t t\<close>
+  assume \<open>cq_map_rel s s\<close>
+  assume \<open>cq_map_rel t t\<close>
   then have bdd_t: \<open>bdd_above (range (kraus_family_norm \<circ> t))\<close>
-    by (auto simp: program_semantics_rel_def)
+    by (auto simp: cq_map_rel_def)
   have inj: \<open>inj_on fst (Set.filter (\<lambda>(E, x). x = f) X)\<close> for X f
     by (auto intro!: inj_onI)
   from bdd_t have bdd': \<open>bdd_above (range (kraus_family_norm \<circ> (\<lambda>e. kraus_family_filter (\<lambda>f. f = c) (t e))))\<close>
@@ -320,9 +318,9 @@ proof (transfer, intro ext)
       using assms by (auto intro!: kraus_family_map_bounded_pos simp add: kraus_family_map'_def)
     also have \<open>\<dots> \<le> 1 * norm (\<rho> d)\<close>
       apply (rule mult_right_mono)
-      using \<open>program_semantics_rel s s\<close>
+      using \<open>cq_map_rel s s\<close>
         kraus_family_norm_filter[of \<open>\<lambda>x. x = f\<close> \<open>s d\<close>]
-       apply (auto intro!: simp: program_semantics_rel_def)
+       apply (auto intro!: simp: cq_map_rel_def)
       by (smt (verit, del_insts))
     also have \<open>\<dots> \<le> norm (\<rho> d)\<close>
       by simp
@@ -371,7 +369,7 @@ proof (transfer, intro ext)
             simp: kraus_family_map'_def kraus_family_map_pos)
       also have \<open>\<dots> \<le> 1 * norm (kraus_family_map' {f} (s d) (\<rho> d))\<close>
         apply (rule mult_right_mono)
-         apply (smt (verit, best) \<open>program_semantics_rel t t\<close> kraus_family_norm_filter program_semantics_rel_def)
+         apply (smt (verit, best) \<open>cq_map_rel t t\<close> kraus_family_norm_filter cq_map_rel_def)
         by simp
       finally show ?thesis
         by simp
@@ -428,23 +426,23 @@ proof (transfer, intro ext)
 qed
 
 
-lemma program_semantics_seq_id_right[simp]: \<open>program_semantics_seq s program_semantics_id = s\<close>
-  apply (rule program_semantics_eqI)
-  by (simp add: program_semantics_apply_seq)
+lemma cq_map_seq_id_right[simp]: \<open>cq_map_seq s cq_map_id = s\<close>
+  apply (rule cq_map_eqI)
+  by (simp add: cq_map_apply_seq)
 
-lemma program_semantics_seq_id_left[simp]: \<open>program_semantics_seq program_semantics_id s = s\<close>
-  apply (rule program_semantics_eqI)
-  by (simp add: program_semantics_apply_seq)
+lemma cq_map_seq_id_left[simp]: \<open>cq_map_seq cq_map_id s = s\<close>
+  apply (rule cq_map_eqI)
+  by (simp add: cq_map_apply_seq)
 
 
-lift_definition program_semantics_if :: \<open>('cl \<Rightarrow> bool) \<Rightarrow> ('cl,'qu) program_semantics \<Rightarrow> ('cl,'qu) program_semantics \<Rightarrow> ('cl,'qu) program_semantics\<close> is
+lift_definition cq_map_if :: \<open>('cl \<Rightarrow> bool) \<Rightarrow> ('cl,'qu) cq_map \<Rightarrow> ('cl,'qu) cq_map \<Rightarrow> ('cl,'qu) cq_map\<close> is
   \<open>\<lambda>e p q c. if e c then p c else q c\<close>
-  by (simp add: program_semantics_rel_def)
+  by (simp add: cq_map_rel_def)
 
-lift_definition program_semantics_quantum_op :: \<open>('cl \<Rightarrow> ('qu ell2, 'qu ell2, unit) kraus_family) \<Rightarrow> ('cl,'qu) program_semantics\<close> is
+lift_definition cq_map_quantum_op :: \<open>('cl \<Rightarrow> ('qu ell2, 'qu ell2, unit) kraus_family) \<Rightarrow> ('cl,'qu) cq_map\<close> is
   \<open>\<lambda>(\<EE>::'cl \<Rightarrow> ('qu ell2, 'qu ell2, unit) kraus_family) c. 
       kraus_family_map_outcome (\<lambda>_. c) (if kraus_family_norm (\<EE> c) \<le> 1 then \<EE> c else 0)\<close>
-  by (simp add: program_semantics_rel_def)
+  by (simp add: cq_map_rel_def)
 
 
 
